Reorganisation.

coq-osiris/examples/proofs/splay.v
@@ -21,6 +21,8 @@ Notation "'Environment'  'composed'  'of'  [ x ; .. ; z ]" :=
 
 (* Boilerplate: reflect the algebraic data type ['a tree]. *)
 
+Local Transparent encode.
+
 Inductive tree (A : Type) : Type :=
 | Leaf: tree A
 | Node: tree A → A → tree A → tree A.
@@ -114,8 +116,7 @@ Proof.
   intros; subst.
   destruct t.
   { eapply pat_consequence_psi.
-    { eapply pat_PData_eq; eapply pat_PTuple.
-      pats. }
+    { eapply pat_PData_eq; pat_PTuple; pats. }
     tauto. }
   { eapply pat_consequence_psi.
     { eapply pat_PData_neq; done. }
@@ -147,8 +148,7 @@ Proof.
   destruct t; eapply pat_consequence_psi.
   { eapply pat_PData_neq; eauto. }
   { tauto. }
-  { eapply pat_PData_eq; eapply pat_PTuple.
-    pats; subst; eauto. }
+  { eapply pat_PData_eq; pat_PTuple; pats; eauto. }
   { clear; right; do 3 eexists; split; [reflexivity | tauto]. }
 Qed.
 
@@ -237,8 +237,7 @@ Proof.
   intros; subst.
   destruct z.
   { eapply pat_consequence_psi.
-    { eapply pat_PData_eq; eapply pat_PTuple.
-      pats. }
+    { eapply pat_PData_eq; pat_PTuple; pats. }
     tauto. }
   { eapply pat_consequence_psi.
     { eapply pat_PData_neq; done. }
@@ -270,8 +269,7 @@ Proof.
   destruct z; eapply pat_consequence_psi.
   { eapply pat_PData_neq; eauto. }
   { tauto. }
-  { eapply pat_PData_eq; eapply pat_PTuple.
-    pats; subst; eauto. }
+  { eapply pat_PData_eq; pat_PTuple; pats; eauto. }
   { clear; do 2 right; do 3 eexists; split; [reflexivity | tauto]. }
   { eapply pat_PData_neq; eauto. }
   { right; left; eauto. }
@@ -301,13 +299,14 @@ Proof.
   { tauto. }
   { eapply pat_PData_neq; eauto. }
   { right; left; eauto. }
-  { eapply pat_PData_eq; eapply pat_PTuple.
-    pats. }
+  { eapply pat_PData_eq; pat_PTuple; pats. }
   { clear; right; right; do 3 eexists; split; [ reflexivity | tauto]. }
 Qed.
 
 Ltac pat_pNodeR :=
   eapply pat_pNodeR; first solve [encode].
+
+Local Opaque encode.
 
 (* -------------------------------------------------------------------------- *)
 
@@ -499,17 +498,6 @@ Proof.
   intros. rewrite Z.ltb_ge. lia.
 Qed.
 
-Lemma pat_consequence_phi η p v (φ φ' : env -> Prop) ψ :
-  (∀ η, φ' η -> φ η) ->
-  pattern η p v φ' ψ ->
-  pattern η p v φ ψ.
-Proof.
-  intros.
-  eapply pat_consequence; eauto.
-Qed.
-
-Opaque encode.
-
 Lemma pure_eval_quadruple `{Encode A1, Encode A2, Encode A3, Encode A4} (η : env) (e1 e2 e3 e4 : expr)
   (ψ : A1 * A2 * A3 * A4 → Prop) :
   pure (eval η e1) (λ a1 : A1,
@@ -522,6 +510,10 @@ Proof.
   intros.
   repeat (let h := fresh in destruct_pure h).
   eapply pure_simp; [ simp | ].
+  eapply pure_simp.
+  { eapply simp_bind.
+    apply simp_evals; eauto. }
+  rewrite bind_ret.
   by pure_ret.
 Qed.
 
@@ -533,30 +525,6 @@ Ltac pattern_hook ::=
     | pat_pLeaf; intros
     | pat_pNode; intros
     ].
-(* -------------------------------------------------------------------------- *)
-(* Specification structures. *)
-
-(* Given a name which corresponds to the declaration, there is some pspec *)
-Class decl_spec (name : var) := { Decl_spec : pspec }.
-
-(* Smart constructor *)
-Definition val_spec (name : var) `{decl_spec name} (v : val) : Prop :=
-  @Decl_spec name _ v.
-
-(* Lifting specification over declaration to a specification over an environment:
-    i.e. the declaration can be found the environment and satisfies the
-    specification. *)
-Definition spec (name : var) `{decl_spec name} (η : env) : Prop :=
-  let val_spec := @Decl_spec name _ in
-  pure (lookup_name η name) val_spec.
-
-(* -------------------------------------------------------------------------- *)
-(* Specification of [splay]. *)
-
-(* Names for the functions we would like to specify *)
-Definition SPLAY := "splay".
-Definition SPLAY_LEAF := "splay_leaf".
-Definition ZLOOKUP := "zlookup".
 
 (* Specification for each function *)
 Definition splay_spec :=
@@ -585,308 +553,247 @@ Definition zlookup_spec :=
           member le x (fringe t) oy ∧
           fringe t' = fringe (fill ctx t)).
 
-#[local] Instance splay_decl_spec : decl_spec SPLAY :=
-  {| Decl_spec := splay_spec |}.
-
-#[local] Instance splay_leaf_decl_spec : decl_spec SPLAY_LEAF :=
-  {| Decl_spec := splay_leaf_spec |}.
-
-#[local] Instance zlookup_decl_spec : decl_spec ZLOOKUP :=
-  {| Decl_spec := zlookup_spec |}.
-
 (* -------------------------------------------------------------------------- *)
+
+(* Specification of [splay]. *)
+
+Section splay_proofs.
 
 (* Top-level environment of [splay]. *)
 
-Definition stdlib_env := ("Stdlib", Stdlib) :: Stdlib_env.
-
-(* Ltac programming to compute the environment from [mexpr]'s. *)
-
-(* Instantiates an evar and tries to apply the aggressive [simp_really] resolution
-   spitting out a [micro] monad if it succeeds. *)
-Ltac try_reduce_with_simp A E m :=
-  let e := fresh "e" in
-  let H := fresh "H" in
-  evar (e : micro A E);
-  assert (H:simp m ?e) by simp_really;
-  clear H;
-  exact e.
-
-(* Given a module definition that has been evaluated, return the environment that
- is built from the evaluated module. *)
-Ltac extract_env module_def :=
-  let m := fresh "m" in
-  let l := fresh "l" in
-  pose module_def as m;
-  unfold module_def in m;
-  match goal with
-  | m := ret (VStruct ?x) |- _ => pose x as l
-  end; clear m; cbn in *; exact l.
-
-(* We can extract the environment programmatically. *)
-Definition splay_module_env' :=
-  (ltac:(try_reduce_with_simp val void (eval_mexpr stdlib_env __main))).
-(* A more sane approach would be to state some well-formedness conditions *)
-
-(* Extracted environment *)
-Definition splay_module_env : env :=
-  ltac:(extract_env splay_module_env').
-
-(* -------------------------------------------------------------------------- *)
-
-(* Util functions for specs *)
-Ltac start_proof := unfold spec; cbn; pure1; red.
-
-(* If a specification holds for an environment, we know that there exists some
-   declaration in the environment that satisfies the specification. *)
-(* TODO fp: It seems to me that this lemma goes too far.
-        It essentially expands away the judgement
-        [pure (lookup_name η name) val_spec]
-        but we should we able to exploit this judgement
-        without expanding it. *)
-Lemma invert_spec :
-  forall x `{decl_spec x} env,
-    spec x env ->
-    ∃ v, lookup_name env x = ret v /\ val_spec x v.
+Lemma Splay_spec :
+  splay_spec
+    (VCloRec stdlib_env [RecBinding "splay" (AnonFunction __branches1)] "splay").
 Proof.
-  intros x Spec env; revert x Spec.
-  induction env.
-  intros * Hspec. red in Hspec; cbn in Hspec.
-  - unfold lookup_name in Hspec.
-    destruct Hspec as (?&Hspec&?).
-    with_strategy transparent [missing_variable_or_field]
-      unfold missing_variable_or_field in Hspec.
-    clarify_simp.
-  - intros * Hspec. red in Hspec.
-    unfold lookup_name in *. destruct a.
-    destruct (x =? v)%string.
-    + destruct Hspec as (?&?&Hspec). clarify_simp.
-      eexists; split; eauto.
-    + fold lookup_name in *. eapply IHenv; eauto.
+  unfold splay_spec.
+  intros A H ctx l x r.
+  (* TODO: Add the following pattern into pure_rec_call *)
+  remember (l, x, r, ctx) as t.
+  replace ctx with t.2 by (rewrite Heqt; reflexivity).
+  replace l with (t.1.1.1) by (rewrite Heqt; reflexivity).
+  replace x with (t.1.1.2) by (rewrite Heqt; reflexivity).
+  replace r with (t.1.2) by (rewrite Heqt; reflexivity).
+  pure_rec t (fun _ : (tree A * A * tree A * zipper A) => True) (@splay_wf A).
+
+  clear l ctx x r.
+  destruct t as [[[l x] r] ctx]; simpl; rename vf into splay.
+
+  (* Match to destruct the argument tuple *)
+  eapply pure_eval_match. { pure_path. reflexivity. }
+  unfold __branches1; pure_match.
+
+  (* Match on [ctx] *)
+  eapply pure_eval_match. { pure_path. reflexivity. }
+  unfold __branches0; pure_match. (* Was very slow, now just slow *)
+
+  (* Case: [ctx] matches [Root] *)
+  { pure_data.
+    prove_same_fringe. }
+
+  (* Case: [ctx] matches [NodeL (Root, y, ry)] *)
+  { pure_data.
+    prove_same_fringe. }
+
+  (* Case: [ctx] matches [NodeL (NodeL (up, z, rz), y, ry)] *)
+  { eapply pure_eval_app. pure_path.
+    eapply pure_eval_quadruple. pure_path. pure_path. pure_data. pure_path.
+    pure_call.
+    { eapply IH; unfold zlt; subst; auto with arith. }
+    simpl; intros ? ->.
+    prove_same_fringe. }
+
+  (* Case: [ctx] matches [NodeL (NodeR (lz, z, up), y, ry)] *)
+  { eapply pure_eval_app. pure_path.
+    eapply pure_eval_quadruple. pure_data. pure_path. pure_data. pure_path.
+    pure_call.
+    { eapply IH; unfold zlt; subst; auto with arith. }
+    intros ? ->.
+    prove_same_fringe. }
+
+  (* Case: [ctx] matches [NodeR (ly, y, Root)] *)
+  { pure_data.
+    prove_same_fringe. }
+
+  (* Case: [ctx] matches [NodeR (ly, y, NodeL (up, z, rz))] *)
+  { eapply pure_eval_app.
+    pure_path.
+    eapply pure_eval_quadruple. pure_data. pure_path. pure_data. pure_path.
+    pure_call.
+    { eapply IH; unfold zlt; subst; auto with arith. }
+    intros ? ->.
+    prove_same_fringe. }
+
+  (* Case: [ctx] matches [NodeR (ly, y, NodeR (lz, z, up))] *)
+  { eapply pure_eval_app. pure_path.
+    eapply pure_eval_quadruple. pure_data. pure_path. pure_path. pure_path.
+    pure_call.
+    { eapply IH; unfold zlt; subst; auto with arith. }
+    intros ? ->.
+    prove_same_fringe. }
 Qed.
 
-(* Apply the specification of a function *)
-Ltac apply_spec SPEC :=
-  let H := fresh "H" in
-  let vspec := fresh "vspec" in
-  let Hlu := fresh "Hlu" in
-  pose proof (invert_spec _ _ SPEC) as H;
-  destruct H as (?&Hlu&vspec);
-  inversion Hlu; subst;
-  try solve [eapply vspec];
-  try (eapply pure_consequence ; first eapply vspec).
 
-(* -------------------------------------------------------------------------- *)
-(* Specification of [splay]. *)
-Section splay_proofs.
+Lemma Splay_leaf_spec splay :
+  splay_spec splay ->
+  splay_leaf_spec
+    (VClo ("splay" ~> splay; stdlib_env) __fun4).
+Proof.
+  unfold splay_leaf_spec.
+  intros Hsplay A H ctx.
+  pure_call_VClo.
+  (* Match on [ctx] *)
+  eapply pure_eval_match. { pure_path; reflexivity. }
+  unfold __branches3; pure_match.
 
-  Notation splay_spec x := (spec x splay_module_env).
+  (* Case: [ctx] matches [Root] *)
+  { pure_const. by subst. }
 
-  Lemma Splay_spec : splay_spec SPLAY.
-  Proof.
-    start_proof.
+  (* Case: [ctx] matches [NodeL (up, x, r)] *)
+  { eapply pure_eval_app. pure_path. (* What does [pure_path] do? *)
+    eapply pure_eval_quadruple.
+    eapply pure_eval_const.
+    apply (@solve_encode_Leaf A); first done. (* Todo: weird *)
+    repeat pure_path.
+    apply Hsplay. }
 
-    repeat intro.
-    (* TODO: Add the following pattern into pure_rec_call *)
-    remember (l, x, r, ctx) as t.
-    replace ctx with t.2 by (rewrite Heqt; reflexivity).
-    replace l with (t.1.1.1) by (rewrite Heqt; reflexivity).
-    replace x with (t.1.1.2) by (rewrite Heqt; reflexivity).
-    replace r with (t.1.2) by (rewrite Heqt; reflexivity).
-    pure_rec t (fun _ : (tree A * A * tree A * zipper A) => True) (@splay_wf A).
+  (* Case: [ctx] matches [NodeR (l, x, up)] *)
+  { eapply pure_eval_app. pure_path. eapply pure_eval_quadruple.
+    pure_path. pure_path. eapply pure_eval_const.
+    apply (@solve_encode_Leaf A). reflexivity.
+    pure_path.
+    apply Hsplay. }
+Qed.
 
-    clear l ctx x r.
-    destruct t as [[[l x] r] ctx]; simpl; rename vf into splay.
+Lemma Zlookup_spec splay splay_leaf :
+  splay_leaf_spec splay_leaf ->
+  splay_spec splay ->
+  zlookup_spec
+    (VCloRec ("splay_leaf" ~> splay_leaf;
+              "splay" ~> splay;
+              stdlib_env)
+       [RecBinding "zlookup" (AnonFunction __branches11)]
+       "zlookup").
+Proof.
+  unfold zlookup_spec.
+  intros Hsplay_leaf Hsplay A H le ? Hcompare t x ctx Hbst.
+  remember (t, x, ctx) as tup eqn:Heqtup.
+  replace ctx with (tup.2) by (rewrite Heqtup; reflexivity).
+  replace x with (tup.1.2) by (rewrite Heqtup; reflexivity).
+  replace t with (tup.1.1) in Hbst |- * by (rewrite Heqtup; reflexivity).
+  pure_rec tup (λ (t : tree A * A * zipper A),
+      match t with
+      | (t, _, _) => bst (strict le) t
+      end) (@zlookup_wf A).
+  repeat (destruct tup as [tup ?]); simpl in *.
+  (* Match on tuple argument *)
+  eapply pure_eval_match. { pure_path. reflexivity. }
+  unfold __branches11; pure_match.
+  (* Match on [t] *)
+  eapply pure_eval_match. { pure_path. reflexivity. }
+  unfold __branches10; pure_match.
 
-    (* Match to destruct the argument tuple *)
-    eapply pure_eval_match. { pure_path. reflexivity. }
-    unfold __branches1; pure_match.
+  (* Case: [t] matches [Leaf] *)
+  { eapply pure_eval_pair. pure_const.
+    eapply pure_eval_app. do 2 pure_path.
+    pure_call.
+    split; [ intros | done]; apply not_elem_of_nil. }
 
-    (* Match on [ctx] *)
-    eapply pure_eval_match. { pure_path. reflexivity. }
-    unfold __branches0; pure_match. (* Was very slow, now just slow *)
+  (* Case: [t] matches [Node (l, y, r)] *)
+  { destruct_bst_Node.
+    eapply pure_eval_let.
+    { (* Evaluate rhs of [let c = ..] *)
+      eapply pure_eval_app2.
+      { pure_path; reflexivity. }
+      { pure_path; reflexivity. }
+      { pure_path; reflexivity. }
+      apply Hcompare. }
+    (* Evaluate continuation expression after let *)
+    intros c (?&Hlt&Heq&Hgt).
+    unfold __exp9.
+    eapply pure_eval_ifthenelse.
+    { (* Evalute comparison operation *)
+      eapply pure_eval_EOpLt.
+      { pure_path. reflexivity. }
+      { eapply pure_eval_int. reflexivity. }
+      { assumption. }
+      { representable. } }
 
-    (* Case: [ctx] matches [Root] *)
-    { pure_data.
-      prove_same_fringe. }
-
-    (* Case: [ctx] matches [NodeL (Root, y, ry)] *)
-    { pure_data.
-      prove_same_fringe. }
-
-    (* Case: [ctx] matches [NodeL (NodeL (up, z, rz), y, ry)] *)
-    { eapply pure_eval_app. pure_path.
-      eapply pure_eval_quadruple. pure_path. pure_path. pure_data. pure_path.
+    { (* Case: [c < 0] *)
+      intro Clt0. unfold __exp5.
+      eapply pure_eval_app. pure_path.
+      eapply pure_eval_triple. pure_path. pure_path. pure_data.
       pure_call.
-      { eapply IH; unfold zlt; subst; auto with arith. }
-      simpl; intros ? ->.
-      prove_same_fringe. }
+      { eapply IH; unfold tlt, tree_depth; auto with arith. }
+      intros [oy t'] [??]; simpl in *.
+      split.
+      - rewrite bst_member_left; representable.
+      - assumption. }
 
-    (* Case: [ctx] matches [NodeL (NodeR (lz, z, up), y, ry)] *)
-    { eapply pure_eval_app. pure_path.
-      eapply pure_eval_quadruple. pure_data. pure_path. pure_data. pure_path.
-      pure_call.
-      { eapply IH; unfold zlt; subst; auto with arith. }
-      intros ? ->.
-      prove_same_fringe. }
-
-    (* Case: [ctx] matches [NodeR (ly, y, Root)] *)
-    { pure_data.
-      prove_same_fringe. }
-
-    (* Case: [ctx] matches [NodeR (ly, y, NodeL (up, z, rz))] *)
-    { eapply pure_eval_app.
-      pure_path.
-      eapply pure_eval_quadruple. pure_data. pure_path. pure_data. pure_path.
-      pure_call.
-      { eapply IH; unfold zlt; subst; auto with arith. }
-      intros ? ->.
-      prove_same_fringe. }
-
-    (* Case: [ctx] matches [NodeR (ly, y, NodeR (lz, z, up))] *)
-    { eapply pure_eval_app. pure_path.
-      eapply pure_eval_quadruple. pure_data. pure_path. pure_path. pure_path.
-      pure_call.
-      { eapply IH; unfold zlt; subst; auto with arith. }
-      intros ? ->.
-      prove_same_fringe. }
-  Qed.
-
-  Lemma Splay_leaf_spec : splay_spec SPLAY_LEAF.
-  Proof.
-    start_proof.
-
-    repeat intro.
-    pure_call_VClo.
-    (* Match on [ctx] *)
-    eapply pure_eval_match. { pure_path; reflexivity. }
-    unfold __branches3; pure_match.
-
-    (* Case: [ctx] matches [Root] *)
-    { pure_const. by subst. }
-
-    (* Case: [ctx] matches [NodeL (up, x, r)] *)
-    { eapply pure_eval_app. pure_path. (* What does [pure_path] do? *)
-      eapply pure_eval_quadruple.
-      eapply pure_eval_const.
-      apply (@solve_encode_Leaf A); first done. (* Todo: weird *)
-      repeat pure_path.
-      apply_spec Splay_spec. }
-
-    (* Case: [ctx] matches [NodeR (l, x, up)] *)
-    { eapply pure_eval_app. pure_path. eapply pure_eval_quadruple.
-      pure_path. pure_path. eapply pure_eval_const.
-      apply (@solve_encode_Leaf A). reflexivity.
-      pure_path.
-      apply_spec Splay_spec. }
-  Qed.
-
-  Lemma Zlookup_spec : splay_spec ZLOOKUP.
-  Proof.
-    start_proof.
-    intros ????.
-    intros Hcompare ??? Hbst.
-    remember (t, x, ctx) as tup eqn:Heqtup.
-    replace ctx with (tup.2) by (rewrite Heqtup; reflexivity).
-    replace x with (tup.1.2) by (rewrite Heqtup; reflexivity).
-    replace t with (tup.1.1) in Hbst |- * by (rewrite Heqtup; reflexivity).
-    pure_rec tup (λ (t : tree A * A * zipper A),
-        match t with
-        | (t, _, _) => bst (strict le) t
-        end) (@zlookup_wf A).
-    repeat (destruct tup as [tup ?]); simpl in *.
-    (* Match on tuple argument *)
-    eapply pure_eval_match. { pure_path. reflexivity. }
-    unfold __branches11; pure_match.
-    (* Match on [t] *)
-    eapply pure_eval_match. { pure_path. reflexivity. }
-    unfold __branches10; pure_match.
-
-    (* Case: [t] matches [Leaf] *)
-    { eapply pure_eval_pair. pure_const.
-      eapply pure_eval_app. do 2 pure_path.
-      apply_spec Splay_leaf_spec.
-      split; [ intros | done]; apply not_elem_of_nil. }
-
-    (* Case: [t] matches [Node (l, y, r)] *)
-    { destruct_bst_Node.
-      eapply pure_eval_let.
-      { (* Evaluate rhs of [let c = ..] *)
-        eapply pure_eval_app2.
-        { pure_path; reflexivity. }
-        { pure_path; reflexivity. }
-        { pure_path; reflexivity. }
-        apply Hcompare. }
-      (* Evaluate continuation expression after let *)
-      intros c (?&Hlt&Heq&Hgt).
-      unfold __exp9.
+    { (* Case: [c >= 0] *)
+      intros Cge0. unfold __exp8.
       eapply pure_eval_ifthenelse.
-      { (* Evalute comparison operation *)
-        eapply pure_eval_EOpLt.
+      { (* Evaluate second comparison operation *)
+        eapply pure_eval_EOpGt.
         { pure_path. reflexivity. }
         { eapply pure_eval_int. reflexivity. }
         { assumption. }
         { representable. } }
 
-      { (* Case: [c < 0] *)
-        intro Clt0. unfold __exp5.
+      { (* Subcase: [c > 0] *)
+        intros Cgt0. unfold __exp6.
         eapply pure_eval_app. pure_path.
         eapply pure_eval_triple. pure_path. pure_path. pure_data.
         pure_call.
-        { eapply IH; unfold tlt, tree_depth; auto with arith. }
+        { eapply IH; [ auto | unfold tlt, tree_depth; lia ]. }
         intros [oy t'] [??]; simpl in *.
         split.
-        - rewrite bst_member_left; representable.
+        - rewrite bst_member_right; representable.
+          by apply Hgt; apply Z.gt_lt.
         - assumption. }
 
-      { (* Case: [c >= 0] *)
-        intros Cge0. unfold __exp8.
-        eapply pure_eval_ifthenelse.
-        { (* Evaluate second comparison operation *)
-          eapply pure_eval_EOpGt.
-          { pure_path. reflexivity. }
-          { eapply pure_eval_int. reflexivity. }
-          { assumption. }
-          { representable. } }
+      { (* Subcase: [c <= 0] *)
+        intros Cle0. unfold __exp7.
+        (* Deduce [c = 0] *)
+        assert (equivalent le a a0) by (apply Heq; lia).
+        eapply pure_eval_pair. pure_data.
+        eapply pure_eval_app. pure_path.
+        eapply pure_eval_quadruple. do 4 pure_path.
+        pure_call.
+        intros. split; first split.
+        - assumption.
+        - apply elem_of_app; right; apply elem_of_cons; by left.
+        - assumption. } } }
+Qed.
 
-        { (* Subcase: [c > 0] *)
-          intros Cgt0. unfold __exp6.
-          eapply pure_eval_app. pure_path.
-          eapply pure_eval_triple. pure_path. pure_path. pure_data.
-          pure_call.
-          { eapply IH; [ auto | unfold tlt, tree_depth; lia ]. }
-          intros [oy t'] [??]; simpl in *.
-          split.
-          - rewrite bst_member_right; representable.
-            by apply Hgt; apply Z.gt_lt.
-          - assumption. }
-
-        { (* Subcase: [c <= 0] *)
-          intros Cle0. unfold __exp7.
-          (* Deduce [c = 0] *)
-          assert (equivalent le a a0) by (apply Heq; lia).
-          eapply pure_eval_pair. pure_data.
-          eapply pure_eval_app. pure_path.
-          eapply pure_eval_quadruple. do 4 pure_path.
-          apply_spec Splay_spec.
-          intros. split; first split.
-          - assumption.
-          - apply elem_of_app; right; apply elem_of_cons; by left.
-          - assumption. } } }
-  Qed.
-
-  Lemma Splay__spec:
-    let η := ("Stdlib", Stdlib) :: Stdlib_env in
-    pure (eval_mexpr η __main)
-      (is_module_with_pspecs [(SPLAY, splay.splay_spec);
-                              (SPLAY_LEAF, splay.splay_leaf_spec);
-                              (ZLOOKUP, splay.zlookup_spec)]).
-  Proof.
-    intros; pure1; simpl.
-    split; last split; red.
-    { apply_spec Splay_spec. }
-    { apply_spec Splay_leaf_spec. }
-    { apply_spec Zlookup_spec. }
-  Qed.
+Lemma Splay__spec:
+  toplevel __main
+    (env_has_pspecs [("splay", splay_spec);
+                            ("splay_leaf", splay_leaf_spec);
+                            ("zlookup", zlookup_spec)]).
+Proof.
+  apply module_struct.
+  eapply structs_cons.
+  { eapply struct_letrec_single.
+    apply Splay_spec. }
+  intros [??] (splay & Hsplay & -> & ->).
+  eapply structs_cons.
+  { eapply struct_let_single.
+    rewrite eval_eval'; simpl.
+    eapply pure_ret. { rewrite <- solve_encode_val; apply eq_refl. }
+    apply Splay_leaf_spec; assumption. }
+  intros [??] (splay_leaf & Hsplay_leaf & -> & ->).
+  eapply structs_cons.
+  { eapply struct_letrec_single.
+    apply Zlookup_spec; assumption. }
+  intros [??] (zlookup & Hzlookup & -> & ->).
+  eapply structs_cons.
+  { eapply struct_let_single.
+    rewrite eval_eval'; simpl.
+    eapply pure_ret. { rewrite <- !solve_encode_val. apply eq_refl. }
+    apply eq_refl. }
+  intros [??] (lookup & Hlookup & -> & ->).
+  apply structs_nil.
+  simpl. tauto.
+Qed.
 
 End splay_proofs.
