coq-osiris/theories/proofmode/notations.v
@@ -372,7 +372,7 @@ Global Arguments eval _ _%expr_scope.
 (*       format "'[' '--------------------------------------env' '//' e '//' '//' {  Q  } ']'"). *)
 
 (* Notation "Γ '--------------------------------------env' module me { Q }" := *)
-(*   (module Γ me Q) *)
+(*   (eval_module Γ me Q) *)
 (*     (only printing, at level 100, *)
 (*       format "'[' Γ '//' '--------------------------------------env' '//' module  me '//' '//' {  Q  } ']'"). *)
 
