coq-osiris/theories/proofmode/wp_tactics.v
@@ -1,0 +1,791 @@
+From iris.proofmode Require Import base proofmode classes environments.
+From iris.base_logic.lib Require Import fancy_updates.
+From iris.bi Require Import weakestpre.
+From iris.prelude Require Import options.
+Import uPred.
+
+From iris Require Import base_logic.lib.gen_heap.
+
+From osiris Require Import base.
+From osiris.lang Require Import lang.
+From osiris.semantics Require Import semantics.
+From osiris.program_logic Require Import program_logic.
+From osiris.proofmode Require Import simp_tactics specifications.
+
+(* ---------------------------------------------------------------------- *)
+(* Tactics to work on WPs. They mimic those on [is_safe]. *)
+
+Lemma tac_change_goal {Σ: gFunctors} Δ (P Q : iProp Σ) :
+  (P ⊢ Q) →
+  envs_entails Δ P →
+  envs_entails Δ Q.
+Proof.
+  eauto using coq_tactics.tac_eval.
+Qed.
+
+(* [lem] must be of the form (P -∗ Q). Thanks to the tactic notation it can be
+   lemma whose forall quantifiers have been instantiated with [_]. *)
+Ltac tac_change_goal lem :=
+  simple notypeclasses refine (tac_change_goal _ _ _ lem _).
+Tactic Notation "tac_change_goal" uconstr(lem) := (tac_change_goal lem).
+
+(* -------------------------------------------------------------------------- *)
+
+(* Tactics to move forward in the proof. *)
+
+(* NOTE:
+ * - The performance of the calls to [cbn] made by the functions below
+ *   crucially depends on adequate unfolding settings being set for terms
+ *   that can appear in the goal, using the [Arguments] command.
+ *   (Such as [eval] and definition it uses transitively or combinators
+ *   of the monad.)
+ *
+ * TODO:
+-* - we still reduce too much:
+ *   + we reduce under continuations;
+ *   + because we reduce the whole Coq context, we reduce all the Iris
+       hypotheses!
+ * TODO: just apply [wp_simp] and reduce in the subgoal [simp m ?m'].
+
+ * TODO: letting [simp] reduce [Stop CEval _ _] is not satisfactory,
+         as it deprives us from the opportunity of applying the lemma
+         [wp_eval] and eliminating a [later] modality. So, the lemma
+         [wp_eval] should be applied first, when applicable.
+
+ * TODO: blindly applying [wp_bind] is dangerous, as it will duplicate
+         the continuation (therefore the entire rest of the proof!)
+         if the left-hand side of the sequence involves a conditional
+         construct. A more cautious approach is to use
+         [wp_bind_binary] and silently apply this lemma
+         only if we are able to silently solve its first premise. *)
+
+Ltac wp_simp :=
+  lazymatch goal with
+  | |- envs_entails _ $ wp _ _ ?m _ =>
+      iApply wp_simp; first solve [simp];
+      lazymatch goal with
+      | |- envs_entails _ $ wp _ _ m _ =>
+          fail
+      | _ => idtac
+      end
+  end.
+
+Ltac wp_step :=
+  (* The lazymatch stills misses a few cases and should be completed. *)
+  lazymatch goal with
+  | |- envs_entails _ (wp _ _ (ret _) _) =>
+      tac_change_goal (wp_ret _ _ _ _)
+  | |- envs_entails _ (wp _ _ (try _ _ _) _) =>
+      tac_change_goal (wp_try _ _ _ _ _ _)
+  (* | |- envs_entails _ (wp _ _ (Par (ret _) (ret _) _ _) _) => *)
+  (*     tac_change_goal (wp_par_ret_ret _ _ _ _ _ _ _) *)
+  (* | |- envs_entails _ (wp _ _ (Par _ (ret _) _ _) _) => *)
+  (*     tac_change_goal (wp_par_ret_right _ _ _ _ _ _ _) *)
+  (* | |- envs_entails _ (wp _ _ (Par (ret _) _ _ _) _) => *)
+  (*     tac_change_goal (wp_par_ret_left _ _ _ _ _ _ _) *)
+  | |- envs_entails _ (wp _ _ (stop CEval _) _) =>
+      first [ iApply wp_eval
+            | tac_change_goal (wp_eval_ret _ _ _ _ _ _)
+            | tac_change_goal (wp_eval _ _ _ _ _ _ _) ]
+  | |- envs_entails _ (wp _ _ (choose ok ?m2) _) =>
+      tac_change_goal (wp_choose_ok _ _ _ _)
+  | |- envs_entails _ (wp _ _ (bind _ _) _) =>
+      fail "[bind] is no longer simplified by [wp_step]."
+  | _ =>
+      fail "The goal must be a wp to apply [wp_step]."
+  end.
+
+Ltac cbn_term m :=
+  lazymatch m with
+  | Par ?m1 ?m2 ?k ?z =>
+      let m'1 := cbn_term m1 in
+      let m'2 := cbn_term m2 in
+      uconstr:(Par m'1 m'2 k z)
+  | Stop ?c ?x ?k ?z =>
+      let x' := eval cbn in x in uconstr:(Stop c x' k z)
+  | _ => let m' := eval cbn -[encode] in m in uconstr:(m')
+  end.
+
+Ltac wp_cbn :=
+  lazymatch goal with
+  | |- envs_entails _ $ wp _ _ ?m _ =>
+      let m' := cbn_term m in
+      first [
+          progress change m with m'
+        | fail "[wp_cbn] No progress to be made." ]
+  | _ => fail "[wp_cbn] WP goal expected."
+  end.
+
+Local Ltac wp_progress :=
+  first [
+      wp_simp
+    | lazymatch goal with
+      | |- envs_entails _ $ wp _ _ (eval _ ?e) _ =>
+          rewrite eval_eval'; try progress wp_cbn
+      end
+    | wp_cbn (* TODO: better control the reduction strategy. *)
+    | cbn beta
+    ].
+
+Local Ltac wp_setup :=
+  iStartProof;
+  lazymatch goal with
+  | |- envs_entails ?Δ $ wp _ _ _ _ =>
+      let Δ :=
+        eval cbn in (env_to_list
+                       (env_intuitionistic Δ)) in
+      let rec lookforme l :=
+        lazymatch constr:(l) with
+        | [] => idtac
+        | (satisfies_spec ?Λ0 ?v) :: ?t =>
+            let Λ := eval hnf in Λ0 in
+            lazymatch constr:(Λ) with
+            | SpecModule Auto ?l ?P =>
+                lazymatch goal with
+                | _ : pure_spec Λ0 v |- _ => idtac
+                | _ =>
+                    iPoseProof ((satisfies_pure_spec Λ v) with "[$]")
+                    as "%";
+                    change Λ with Λ0 in *
+                end
+            | _ => idtac
+            end ; lookforme t
+        | _ :: ?t => lookforme t
+        end in
+      lookforme Δ
+  end
+.
+
+Ltac wp :=
+  wp_setup;
+  lazymatch goal with
+  | |- envs_entails _ $ wp _ _ (eval (_ ++ _) _) _ =>
+      simpl app
+  | _ => idtac
+  end;
+  repeat
+    (first [
+         (* 1. Try to eliminate a later or take a step. *)
+         lazymatch goal with
+         | |- envs_entails _ $ wp _ _ (eval (_ ++ _) _) _ =>
+             idtac
+         | |- envs_entails _ (bi_later _) => iNext
+         | _ => wp_step
+         end
+       | (* 2. Try to simplify the proof goal using [wp_progress].*)
+         wp_progress
+    ]).
+
+(* [wp_bind] can be applied when the goal is of the form [WP bind m m' {{ _ }}].
+   It bahaves differently depending on the term [m]:
+   - if [m] can be simplified into [ret v], then [bind] can reduce: do it;
+   - otherwise, apply the lemma [wp_bind]. *)
+Ltac wp_bind :=
+  lazymatch goal with
+  | |- envs_entails _ (wp _ _ (bind _ _) _) =>
+      first [
+          (* [wp_simp] will reduce the bind if it can. *)
+          try wp_simp; try iApply wp_bind
+        | tac_change_goal (wp_bind _ _ _ _ _) ]
+  | _ => fail "[wp_bind] should only be applied to goals of the form [WP bind _ _ {{ _ }}]."
+  end; wp.
+
+(* -------------------------------------------------------------------------- *)
+
+(* TODO: get [wp until check _] to use [idtac_or_do]. *)
+Local Tactic Notation "idtac_or_do" constr(name) constr(δ) ltac(t) :=
+  let is_in := eval cbn in (lookup_name δ name) in
+  lazymatch is_in with
+  | @Ret _ void _ => idtac
+  | _ => t
+  end.
+
+Local Tactic Notation "@wp" "until" "check" constr(name) :=
+  lazymatch goal with
+  | |- envs_entails _ $ wp _ _ (ret (?δ ++ _, ?δ ++ _)) _ =>
+      let is_in := eval cbn in (lookup_name δ name) in
+        lazymatch is_in with
+        | @Ret _ void _ => idtac
+        | _ => fail "[wp until] cannot find the requested bindings"
+        end
+  | |- envs_entails _ $ wp _ _ (ret (?δ ++ ?η)) _ =>
+      let is_in := eval cbn in (lookup_name δ name) in
+        lazymatch is_in with
+        | @Ret _ void _ => idtac
+        | _ => fail "[wp until] cannot find the requested bindings"
+        end
+  | _ => fail "[wp until] cannot find the requested bindings."
+  end.
+
+Tactic Notation "@wp" "until" constr(name) :=
+  repeat (
+      first
+        [
+          lazymatch goal with
+          | |- envs_entails _ $ wp _ _ (ret (?δ ++ _, ?δ ++ _)) _ =>
+              idtac_or_do
+                name δ
+                wp
+          | |- envs_entails _ $ wp _ _ (ret (?δ ++ ?η)) _ =>
+              idtac_or_do
+                name δ
+                wp
+          end
+        | wp
+    ]).
+
+Tactic Notation "wp" "until" constr(name) :=
+  @wp until name;
+  first [ @wp until check name
+        | idtac "The requested binding was not found."
+    ].
+
+Tactic Notation "wp" "until" constr(name) "!" :=
+  repeat (@wp until name; try wp_bind);
+  @wp until check name.
+
+(* -------------------------------------------------------------------------- *)
+
+Ltac wp_par :=
+  iApply wp_par; [wp | wp | .. ].
+
+Ltac wp_par_with H :=
+  iApply (wp_par with H); [wp | wp | .. ].
+
+Ltac wp_use H :=
+  first [
+    iApply H
+  | iApply wp_covariant; [ iApply H |]
+  | iApply (wp_covariant with H)
+  ];
+  cbn.
+
+Ltac wp_enter :=
+  iApply wp_simp; [
+    simp_enter; [ normalize; eapply SimpReflexive ]
+  | (* residual goal *)
+  ].
+
+Ltac wp_enter_and_abstract :=
+  lazymatch goal with |- envs_entails _ (wp _ _ (call ?v _) _) =>
+    (* First, expand [call] away. *)
+    iApply wp_simp; [
+      simp_enter; eapply SimpReflexive
+    | normalize
+    ];
+    (* Second, abstract away the closure (of which there are typically
+       several occurrences in the hypotheses and goal), replacing it
+       with an abstract value. This ensures that we cannot step into
+       recursive calls. *)
+    generalize dependent v
+  end.
+
+Ltac wp_pure_postcondition' :=
+  let x := fresh "x" in
+  iIntros (x) "Hψ"; destruct x; [ | done];
+    iDestruct "Hψ" as "%Hψ"; subst; cbn.
+
+Ltac wp_intro_pure :=
+  match goal with
+  | |- envs_entails _ (@bi_forall _ val _) =>
+      let e := fresh "e" in
+      iIntros (e)
+  | |- envs_entails _ (@bi_forall _ outcome _) =>
+      let e := fresh "e" in
+      iIntros (e);
+      try destruct e as [e | e]; last (try (elim_void e))
+  end.
+
+Ltac wp_lift_ipure :=
+  lazymatch goal with
+  | |- envs_entails _ (bi_wand (lift_ipure _ (Res ?e)) _) =>
+      let H := fresh "H" in
+      iIntros "H"; iDestruct "H" as %H
+  end.
+
+Ltac wp_pure_postcondition :=
+  repeat wp_intro_pure; repeat wp_lift_ipure; subst; cbn.
+
+(* TODO: not great *)
+Ltac wp_set_postcondition :=
+    by
+    lazymatch goal with
+    | |- envs_entails _ (@ipure ?res ?exn ?Σ ?φ ?v) =>
+        is_evar φ;
+        let H := eval cbn in (λ R : @outcome res exn,
+                                 ⌜R = @Res res exn v⌝%I : iPropI Σ)%I in
+        instantiate (1 := H)
+    | |- envs_entails ?Δ (?φ ?v) =>
+        is_evar φ;
+        let hyps :=
+          eval cbn in (
+                     env_to_list $
+                     env_spatial Δ
+                   ) in
+        let H := eval cbn in (
+                            match hyps with
+                            | [] => λ res, ⌜ res = v ⌝%I
+                            | _ => (λ res, ⌜ res = v ⌝ ∗ [∗ list] p ∈ hyps, p)%I
+                            end)%I in
+          instantiate (1 := H)
+    end.
+
+Ltac wp_absurd :=
+  by
+    lazymatch goal with
+    | e: void |- _ =>
+        elim_void e
+    | |- envs_entails _ (@bi_forall _ void _) =>
+        let e := fresh "e" in
+        iIntros (e); elim_void e
+    end.
+
+(* -------------------------------------------------------------------------- *)
+
+(* Store-related tactics. *)
+
+Ltac wp_alloc l H:=
+  iApply wp_alloc; iNext; iIntros (l) H; wp.
+Ltac wp_load H :=
+  iApply (wp_load with H); iNext; iIntros H; wp.
+Ltac wp_store H :=
+  iApply (wp_store with H); iNext; iIntros H; wp.
+
+(* -------------------------------------------------------------------------- *)
+(* Tactics used to prove the specification of a module expression. *)
+
+
+Ltac wp_module_spec :=
+  lazymatch goal with
+  | |- envs_entails _  (?φ (VStruct ?η)) =>
+      iExists _; iSplit ; first  (iPureIntro; reflexivity);
+      repeat first
+             [ (iApply big_sepL_cons; iSplitL;
+                first (iExists _; iSplit; [ done | iAssumption || done ])
+               )
+             | iApply big_sepL_nil; iPureIntro; exact I
+             | idtac
+                 "I cannot prove the required spec; please go back and prove the required specifications."
+             ]
+  end.
+
+(* -------------------------------------------------------------------------- *)
+
+(* Help reason on loops of the form [for i = x to y], whth [0 <= x <= y]. *)
+Tactic Notation "oLoopPos" constr(v1) constr(v2) constr(Hinv) "with" constr(Hini) constr(Hend) :=
+  let H := eval cbn in (Hini +:+ Hend) in
+    lazymatch goal with
+    | |- envs_entails
+           _ $
+           wp _ _ (Stop CLoop (?η, ?x, repr ?i1, repr ?i2, ?e) ?k ?z) ?φ =>
+        iApply
+          ((wp_loop_inv_pos NotStuck ⊤ η x v1 v2 e k z φ Hinv)
+            with H);
+        try lia; try representable
+    | _ => fail "[oLoop] can only be applied to terms of the form [WP (Stop CLoop _ _ _) {{ _ }}]"
+    end.
+
+(* -------------------------------------------------------------------------- *)
+
+(* [Ltac] helpers to deal with value abstraction. *)
+
+Tactic Notation "oAbstract" constr(s1) ident(i1):=
+  lazymatch goal with
+  | |- context [VCloRec ?η ?bds s1] =>
+      generalize (VCloRec η bds s1); intro i1
+  | |- context [(s1, (VClo ?η ?e)) :: _] =>
+      generalize (VClo η e); intro i1
+  end.
+Tactic Notation "oAbstract"
+       constr(s1) ident(i1)
+       constr(s2) ident(i2) :=
+  oAbstract s1 i1;
+  oAbstract s2 i2.
+Tactic Notation "oAbstract"
+       constr(s1) ident(i1)
+       constr(s2) ident(i2)
+       constr(s3) ident(i3) :=
+  oAbstract s1 i1;
+  oAbstract s2 i2
+            s3 i3.
+Tactic Notation "oAbstract"
+       constr(s1) ident(i1)
+       constr(s2) ident(i2)
+       constr(s3) ident(i3)
+       constr(s4) ident(i4):=
+  oAbstract s1 i1
+            s2 i2;
+  oAbstract s3 i3
+            s4 i4.
+
+(* -------------------------------------------------------------------------- *)
+
+(* [oCall] behaves in the same way that wp_call does, except that it abstracts
+   the required closures.
+   It is defined as a notation so that it is easy to ask for more idents (Ltac
+   cannot take a list of idents as argument for a tactic). *)
+Tactic Notation "@oCall" "unfold" :=
+  with_strategy
+    transparent [call]
+    ( lazymatch goal with
+      | |- envs_entails ?Δ $ wp ?s ?E (call ?f ?a) ?φ =>
+          let m := eval unfold call in (call f a) in
+            change (envs_entails Δ $ wp s E (call f a) φ)
+              with (envs_entails Δ $ wp s E m φ)
+      | _ => fail "[oCall] The goal is not a call"
+      end); try wp.
+
+Tactic Notation "oCall" constr(s1) ident(i1) :=
+  (* TODO if possible, use [wp_enter] instead of [unfold call] *)
+  @oCall unfold; try wp;
+  lazymatch goal with
+  | |- context [VCloRec ?η ?bds s1] =>
+      generalize (VCloRec η bds s1); intro i1
+  end; try wp.
+Tactic Notation "oCall" constr(s1) ident(i1) constr(s2) ident(i2) :=
+  @oCall unfold; try wp;
+  lazymatch goal with
+  | |- context [VCloRec ?η ?bds s1] =>
+      generalize (VCloRec η bds s1); intro i1
+  end;
+  lazymatch goal with
+  | |- context [VCloRec ?η ?bds s2] =>
+      generalize (VCloRec η bds s2); intro i2
+  end; try wp.
+
+(* -------------------------------------------------------------------------- *)
+
+(* Below are defined local tactics which are used to define [oSpecify]. *)
+
+(* [oSpecify] is used to provide the user the possibility to provide
+   specifications for variables which are about to be added to the environment
+   through [ret_dconcat].
+   The tactic notation only works for two arguments, as it is what is required
+   here. If it works, it should be moved to [proofmode/specifications.v].
+   Note: [ret_dconcat] only takes two arguments now (the continuation is
+         always ret). *)
+Local Ltac oSpecify_intros lnames :=
+  let hyps := eval cbn in (foldr String.append "" lnames) in
+  iIntros hyps.
+
+(* [oSpecify_assume_nonrec specs names hyps δ] assumes specifications of
+   elements of a let-binding. *)
+Local Ltac oSpecify_assume_nonrec lspecs lnames lhyps δ :=
+  let specs :=
+    eval cbn in (
+               foldr
+                 (λ '(spec, name) (res: list (iProp _)),
+                   let value :=
+                     match lookup_name δ name with
+                     | @Ret _ _ v => v
+                     | _ => VUnit
+                     end in
+                   spec value :: res)
+                 [] (combine lspecs lnames)
+             )
+    in
+    iApply (assuming_list_nonrec specs);
+    last oSpecify_intros lhyps.
+
+(* [oSpecify_assume specs names hyps δ] assumes specifications of elements of a
+   letrec-binding. The difference with a let-binding is that
+   Löb-induction-related hypotheses are provided: when proving the spec of
+   mutually recursive functions [f] and [g], the specifications are available
+   under a later modality. This only works for persistent specifications.
+   Cf. [assuming_list] in [theories/proofmode/specifications.v] for more
+   details. *)
+Local Ltac oSpecify_assume lspecs lnames lhyps δ :=
+  let specs :=
+    eval cbn in (
+               foldr
+                 (λ '(spec, name) (res: list (iProp _)),
+                   let value :=
+                     match lookup_name δ name with
+                     | @Ret _ _ v => v
+                     | _ => VUnit
+                     end in
+                   spec value :: res)
+                 [] (combine lspecs lnames)
+             )
+    in
+    iApply (assuming_list specs);
+      first (by eauto using intuitionistically_persistent);
+      (try iModIntro);
+      oSpecify_intros lhyps.
+
+Tactic Notation "oSpecify_abstract" constr(δ) constr(n1) ident(i1) :=
+  let value :=
+    eval cbn in (match lookup_name δ n1 with
+                           | @Ret _ _ v => v
+                           | _ => VUnit
+                           end) in
+    generalize value; intros i1.
+
+Tactic Notation "oSpecify_abstract" constr(δ)
+       constr(n1) ident(i1)
+       constr(n2) ident(i2) :=
+  oSpecify_abstract δ n1 i1;
+  oSpecify_abstract δ n2 i2.
+
+Tactic Notation "oSpecify_abstract" constr(δ)
+       constr(n1) ident(i1)
+       constr(n2) ident(i2)
+       constr(n3) ident(i3) :=
+  oSpecify_abstract δ n1 i1 n2 i2;
+  oSpecify_abstract δ n3 i3.
+
+Tactic Notation "oSpecify_abstract" constr(δ)
+       constr(n1) ident(i1)
+       constr(n2) ident(i2)
+       constr(n3) ident(i3)
+       constr(n4) ident(i4) :=
+  oSpecify_abstract δ n1 i1 n2 i2;
+  oSpecify_abstract δ n3 i3 n4 i4.
+
+(* -------------------------------------------------------------------------- *)
+
+(* Definition of [oSpecify], used to specify and abstract away values when the
+   evaluation stops on en environment concatenation. *)
+
+Tactic Notation "oSpecify"
+       constr(n1) constr(spec1) ident(i1) constr(H1) :=
+  lazymatch goal with
+  | |- envs_entails
+         _ (wp _ _ (eval (?δ ++ _) _) _) =>
+      oSpecify_assume_nonrec [spec1] [n1] [H1] δ;
+      last ( oSpecify_abstract δ n1 i1 )
+  | |- envs_entails
+         _ (wp _ _ (eval (?δ ++ _, ?δ ++ _) _) _) =>
+      oSpecify_assume [spec1] [n1] [H1] δ;
+      last ( oSpecify_abstract δ n1 i1 )
+  | _ => fail "[oSpecify] only works on environment extension."
+  end.
+Tactic Notation "oSpecify"
+       constr(n1) constr(spec1) ident(i1) constr(H1)
+       constr(n2) constr(spec2) ident(i2) constr(H2) :=
+  lazymatch goal with
+  | |- envs_entails
+         _ (wp _ _ (eval (?δ ++ _, ?δ ++ _) _) _) =>
+      oSpecify_assume [spec1; spec2]
+                             [n1; n2]
+                             [H1; H2]
+                             δ;
+      last ( oSpecify_abstract δ n1 i1 n2 i2 )
+  | |- envs_entails
+         _ (wp _ _ (eval (?δ ++ _) _) _) =>
+      oSpecify_assume_nonrec [spec1; spec2]
+                      [n1; n2]
+                      [H1; H2]
+                      δ;
+      last ( oSpecify_abstract δ n1 i1 n2 i2 )
+  | _ => fail "[oSpecify] only works on environment extension."
+  end.
+Tactic Notation "oSpecify"
+       constr(n1) constr(spec1) ident(i1) constr(H1)
+       constr(n2) constr(spec2) ident(i2) constr(H2)
+       constr(n3) constr(spec3) ident(i3) constr(H3) :=
+  lazymatch goal with
+  | |- envs_entails
+         _ (wp _ _ (eval (?δ ++ _) _) _) =>
+      oSpecify_assume_nonrec [spec1; spec2; spec3] [n1; n2; n3] [H1; H2; H3] δ;
+      last ( oSpecify_abstract δ n1 i1 n2 i2 n3 i3 )
+  | |- envs_entails
+         _ (wp _ _ (eval (?δ ++ _, ?δ ++ _) _) _) =>
+      oSpecify_assume [spec1; spec2; spec3] [n1; n2; n3] [H1; H2; H3] δ;
+      last ( oSpecify_abstract δ n1 i1 n2 i2 n3 i3 )
+  | _ => fail "[oSpecify] only works on environment extension."
+  end.
+Tactic Notation "oSpecify"
+       constr(n1) constr(spec1) ident(i1) constr(H1)
+       constr(n2) constr(spec2) ident(i2) constr(H2)
+       constr(n3) constr(spec3) ident(i3) constr(H3)
+       constr(n4) constr(spec4) ident(i4) constr(H4) :=
+  lazymatch goal with
+  | |- envs_entails
+         _ (wp _ _ (eval (?δ ++ _) _) _) =>
+      oSpecify_assume_nonrec [spec1; spec2; spec3; spec4]
+                             [n1; n2; n3; n4]
+                             [H1; H2; H3; H4]
+                             δ;
+      last ( oSpecify_abstract δ n1 i1 n2 i2 n3 i3 n4 i4 )
+  | |- envs_entails
+         _ (wp _ _ (eval (?δ ++ _, ?δ ++ _) _) _) =>
+      oSpecify_assume [spec1; spec2; spec3; spec4]
+                      [n1; n2; n3; n4]
+                      [H1; H2; H3; H4]
+                      δ;
+      last ( oSpecify_abstract δ n1 i1 n2 i2 n3 i3 n4 i4 )
+  | _ => fail "[oSpecify] only works on environment extension."
+  end.
+
+(* -------------------------------------------------------------------------- *)
+
+  (* [list_specifications] returns a list of specifications for a given symbol
+     of a given module specification. *)
+  Definition list_specifications `{Σ: gFunctors}
+           (Λ : @spec_env Σ) (name : name)
+    : list (val → iProp Σ) :=
+    List.map snd $
+             List.filter (fun '(n, _) => n =? name)%string Λ.
+
+Tactic Notation "oSpecOf" constr(name) "from" constr(hyp) "as" constr(hyp_dest) :=
+  lazymatch goal with
+  | |- envs_entails
+         ?Δ $ wp _ _
+         (call ((lookup_name_total (val_as_struct_total ?v) ?n)) _) _ =>
+      (* - [v] stores the value of the module,
+         - [n] stores the name of the symbol (depth 1).
+         The first step is to find the Iris hypothesis discussing the module
+         [v]. *)
+      let env := eval cbn in
+      (env_lookup
+         (INamed hyp) $ env_intuitionistic Δ) in
+      let φs :=
+        lazymatch constr:(env) with
+        | None => fail "Unknown hypothesis"
+        | Some (module_spec ?Λ v) =>
+            eval cbn in (list_specifications Λ name)
+        | _ => fail "The target hypothesis is not a module specification"
+        end in
+      lazymatch constr:(φs) with
+      | [] => fail "There is no specification for" name
+      | [ ?φ ] =>
+          iPoseProof ((module_spec_spec _ _ name) with hyp) as hyp_dest
+      | _ => fail "There are too many specifications to choose from"
+      end
+  | _ => fail "[oSpecOf] could not fild the required specification."
+  end.
+
+Ltac oSpecError name spec :=
+  fail "[oSpec] failed to apply the specification of" name
+       "; Please consider using [oSpecOf " name "from" spec
+       "as ...] to retrieve the spec yourself".
+
+Tactic Notation "oSpec" constr(name) "from" constr(spec) "with" constr(Hyp) :=
+  let H := iFresh in
+  oSpecOf name from spec as H;
+  first [
+      iSpecialize (H with Hyp);
+      last (iApply (wp_covariant with H) ; try iClear H)
+    | oSpecError name spec
+    ]; try wp.
+
+(* Preconditions are often pure and might not need any hypothesis. *)
+Tactic Notation "oSpec" constr(name) "from" constr(spec) :=
+  first [
+      oSpec name from spec with "[//]"
+    | let H := iFresh in
+      oSpecOf name from spec as H;
+      first [
+          iApply (wp_covariant with H);
+          last try iClear H
+        | oSpecError name spec
+        ]
+    | oSpec name from spec with "[]"
+    ].
+
+(* Ditto for [satisfies_spec]... *)
+
+Tactic Notation "oSpecOf'" constr(name) "from" constr(hyp) "as" constr(H) :=
+  iPoseProof ((bloupyfetcher _ _ _ _ name) with hyp) as H
+.
+Tactic Notation "oSpec'" constr(name) "from" constr(spec) "with" constr(Hyp) :=
+  let H := iFresh in
+  oSpecOf' name from spec as H;
+  first [
+      iSpecialize (H with Hyp);
+      last (iApply (wp_covariant with H) ; try iClear H)
+    | oSpecError name spec
+    ]; try wp.
+
+Tactic Notation "oSpec'" constr(name) "from" constr(spec) :=
+  first [
+      oSpec' name from spec with "[//]"
+    | let H := iFresh in
+      oSpecOf' name from spec as H;
+      first [
+          iApply (wp_covariant with H);
+          last try iClear H
+        | oSpecError name spec
+        ]
+    | oSpec' name from spec with "[]"
+    ].
+
+(* -------------------------------------------------------------------------- *)
+
+(* In order for lookups and evaluation of module-values to be evaluated, one
+   needs to declare the value the representation of a module. *)
+Tactic Notation "oModule" ident(v) :=
+  iPoseProof ((module_spec_is_module v) with "[$]") as "%";
+  simpl (spec_env_erase _) in *.
+Tactic Notation "oModule" ident(v1) ident(v2) :=
+  oModule v1; oModule v2.
+Tactic Notation "oModule" ident(v1) ident(v2) ident(v3) :=
+  oModule v1; oModule v2 v3.
+Tactic Notation "oModule" ident(v1) ident(v2) ident(v3) ident(v4) :=
+  oModule v1 v2; oModule v3 v4.
+
+(* -------------------------------------------------------------------------- *)
+
+(* Wrapers around the above [Tactic Notation]s to autoname idents.
+   For some (unknown) reason, it is not possible to overload [oSpecify] with
+   four new notations, even if the arities differ from the previous notations.
+ *)
+
+From iris.proofmode Require Import string_ident.
+
+Tactic Notation "o_specify"
+       constr(n1) constr(spec1) constr(H1) :=
+  string_to_ident_cps n1 ltac:(fun i1 =>
+  let i1 := fresh i1 in
+  oSpecify n1 spec1 i1 H1).
+Tactic Notation "o_specify"
+       constr(n1) constr(spec1) constr(H1)
+       constr(n2) constr(spec2) constr(H2) :=
+  string_to_ident_cps
+    n1
+    ltac:(fun i1 =>
+            let i1 := fresh i1 in
+            string_to_ident_cps
+              n2
+              ltac:(fun i2 =>
+                      let i2 := fresh i2 in
+                      oSpecify n1 spec1 i1 H1
+                               n2 spec2 i2 H2)).
+Tactic Notation "o_specify"
+       constr(n1) constr(spec1) constr(H1)
+       constr(n2) constr(spec2) constr(H2)
+       constr(n3) constr(spec3) constr(H3) :=
+  string_to_ident_cps
+    n1
+    ltac:(fun i1 =>
+            let i1 := fresh i1 in
+            string_to_ident_cps
+              n2
+              ltac:(fun i2 =>
+                      let i2 := fresh i2 in
+                      string_to_ident_cps
+                        n3
+                        ltac:(fun i3 =>
+                                let i3:= fresh i3 in
+                                oSpecify n1 spec1 i1 H1
+                                         n2 spec2 i2 H2
+                                         n3 spec3 i3 H3))).
+
+(* -------------------------------------------------------------------------- *)
+
+(* When using the above tactics in real-life examples, some patterns have
+   emerged. The following tactic notations are shortcuts one may find useful in
+   proofs. *)
+
+Tactic Notation "oSpecify"
+       constr(n1) constr(spec1) ident(i1) constr(H1) "!" :=
+  wp until n1 ! ;
+  oSpecify n1 spec1 i1 H1.
+
+Tactic Notation "wp" "skip" constr(n1) := wp until n1 ! ; wp.
+Tactic Notation "wp" "skip" constr(n1) constr(n2) := wp skip n1 ; wp skip n2.
+Tactic Notation "wp" "skip" constr(n1) constr(n2) constr(n3) :=
+  wp skip n1 ; wp skip n2 n3.
+Tactic Notation "wp" "skip" constr(n1) constr(n2) constr(n3) constr(n4) :=
+  wp skip n1 n2 ; wp skip n3 n4.
